git/leanprover/lean4/src/Lean/Compiler/Simp.lean
@@ -27,124 +27,104 @@ partial def findExpr (e : Expr) (skipMData := true): CompilerM Expr := do
   | .mdata _ e' => if skipMData then findExpr e' else return e
   | _ => return e
 
+inductive Occ where
+  | once
+  | many
+  deriving Repr, Inhabited
+
 /--
 Local function declaration statistics.
 
 Remark: we use the `userName` as the key. Thus, `ensureUniqueLetVarNames`
 must be used before collectin stastistics.
 -/
-structure InlineStats where
+structure OccInfo where
   /--
-  Mapping from local function name to the number of times it is used
-  in a declaration.
+  Mapping from local function name to occurrence information.
   -/
-  numOccs : Std.HashMap Name Nat := {}
-  /--
-  Mapping from local function name to their LCNF size.
-  -/
-  size : Std.HashMap Name Nat := {}
+  map : Std.HashMap Name Occ := {}
+  deriving Inhabited
 
-def InlineStats.format (s : InlineStats) : Format := Id.run do
+def OccInfo.format (s : OccInfo) : Format := Id.run do
   let mut result := Format.nil
-  for (k, n) in s.numOccs.toList do
-    let some size := s.size.find? k | pure ()
-    result := result ++ "\n" ++ f!"{k} ↦ {n}, {size}"
-    pure ()
+  for (k, n) in s.map.toList do
+    result := result ++ "\n" ++ f!"{k} ↦ {repr n}"
   return result
 
-def InlineStats.shouldInline (s : InlineStats) (k : Name) : Bool := Id.run do
-  let some numOccs := s.numOccs.find? k | return false
-  if numOccs == 1 then return true
-  let some sz := s.size.find? k | return false
-  return sz == 1
+instance : ToFormat OccInfo where
+  format := OccInfo.format
 
-instance : ToFormat InlineStats where
-  format := InlineStats.format
-
-partial def collectInlineStats (e : Expr) : CoreM InlineStats := do
-  let ((_, s), _) ← goLambda e |>.run {} |>.run {}
-  return s
-where
-  goLambda (e : Expr) : StateRefT InlineStats CompilerM Unit := do
-    withNewScope do
-      let (_, body) ← visitLambda e
-      go body
-
-  goValue (value : Expr) : StateRefT InlineStats CompilerM Unit := do
-    match value with
-    | .lam .. => goLambda value
-    | .app .. =>
-      match (← findLambda? value.getAppFn) with
-      | some localDecl =>
-        if localDecl.value.isLambda then
-          let key := localDecl.userName
-          match (← get).numOccs.find? localDecl.userName with
-          | some numOccs => modify fun s => { s with numOccs := s.numOccs.insert key (numOccs + 1) }
-          | _ =>
-            let sz ← getLCNFSize localDecl.value
-            modify fun { numOccs, size } => { numOccs := numOccs.insert key 1, size := size.insert key sz }
-      | _ => pure ()
-    | _ => pure ()
-
-  go (e : Expr) : StateRefT InlineStats CompilerM Unit := do
-    match e with
-    | .letE .. =>
-      withNewScope do
-        let body ← visitLet e fun _ value => do goValue value; return value
-        go body
-    | e =>
-      if let some casesInfo ← isCasesApp? e then
-        let args := e.getAppArgs
-        for i in casesInfo.altsRange do
-          goLambda args[i]!
-      else
-        goValue e
+def OccInfo.add (s : OccInfo) (key : Name) : OccInfo :=
+  match s with
+  | { map } =>
+    match map.find? key with
+    | some .once => { map := map.insert key .many }
+    | none       => { map := map.insert key .once }
+    | _          => { map }
 
 structure Config where
-  increaseFactor : Nat := 2
+  smallThreshold : Nat := 1
 
 structure Context where
   config : Config := {}
-  /--
-  Statistics for deciding whether to inline local function declarations.
-  -/
-  stats : InlineStats
-  /--
-  We only inline local declarations when `localInline` is `true`.
-  We set it to `false` when we are inlining a non local definition
-  that may have let-declarations whose names collide with the ones
-  stored at `stats`.
-  -/
-  localInline : Bool := true
 
 structure State where
+  /--
+  (Approximate) occurence information for local function declarations.
+  -/
+  occInfo : OccInfo := {}
   simplified : Bool := false
   deriving Inhabited
 
 abbrev SimpM := ReaderT Context $ StateRefT State CompilerM
 
-structure SavedState where
-  compiler : CompilerM.SavedState
-  simp : State
-  deriving Inhabited
+/-- Ensure binder names are unique, and update occurrence information -/
+partial def internalize (e : Expr) : SimpM Expr := do
+  visitLambda e
+where
+  visitLambda (e : Expr) : SimpM Expr := do
+    withNewScope do
+      let (as, e) ← Compiler.visitLambda e
+      let e ← mkLetUsingScope (← visitLet e #[])
+      mkLambda as e
 
-protected def saveState : SimpM SavedState :=
-  return { compiler := (← CompilerM.saveState), simp := (← get) }
+  visitCases (casesInfo : CasesInfo) (cases : Expr) : SimpM Expr := do
+    let mut args := cases.getAppArgs
+    for i in casesInfo.altsRange do
+      args ← args.modifyM i visitLambda
+    return mkAppN cases.getAppFn args
 
-/-- Restore backtrackable parts of the state. -/
-def SavedState.restore (b : SavedState) : SimpM Unit := do
-  b.compiler.restore
-  set b.simp
+  visitValue (e : Expr) : SimpM Unit := do
+    if e.isApp then
+      match (← findLambda? e.getAppFn) with
+      | some localDecl =>
+        if localDecl.value.isLambda then
+          let key := localDecl.userName
+          modify fun s => { s with occInfo := s.occInfo.add key  }
+      | _ => pure ()
 
-instance : MonadBacktrack SavedState SimpM where
-  saveState      := Simp.saveState
-  restoreState s := s.restore
-
-def withLocalInline (localInline : Bool) (x : SimpM α) : SimpM α :=
-  withReader (fun ctx => { ctx with localInline }) x
-
-def withoutLocalInline (x : SimpM α) : SimpM α :=
-  withLocalInline false x
+  visitLet (e : Expr) (xs : Array Expr) : SimpM Expr := do
+    match e with
+    | .letE binderName type value body nonDep =>
+      let idx ← mkFreshLetVarIdx
+      let binderName' := match binderName with
+        | .num p _ => .num p idx
+        | _ => .num binderName idx
+      let type  := type.instantiateRev xs
+      let mut value := value.instantiateRev xs
+      if value.isLambda then
+        value ← visitLambda value
+      else
+        visitValue value
+      let x ← mkLetDecl binderName' type value nonDep
+      visitLet body (xs.push x)
+    | _  =>
+      let e := e.instantiateRev xs
+      if let some casesInfo ← isCasesApp? e then
+        visitCases casesInfo e
+      else
+        visitValue e
+        return e
 
 def markSimplified : SimpM Unit :=
   modify fun s => { s with simplified := true }
@@ -160,6 +140,7 @@ def simpProj? (e : Expr) : OptionT SimpM Expr := do
   let .proj _ i s := e | failure
   let s ← findCtor s
   let some (ctorVal, args) := s.constructorApp? (← getEnv) | failure
+  markSimplified
   return args[ctorVal.numParams + i]!
 
 /--
@@ -176,10 +157,13 @@ def simpAppApp? (e : Expr) : OptionT SimpM Expr := do
   guard f.isFVar
   let f ← findExpr f
   guard <| f.isApp || f.isConst
+  markSimplified
   return mkAppN f e.getAppArgs
 
-def shouldInline (localDecl : LocalDecl) : SimpM Bool :=
-  return (← read).localInline && (← read).stats.shouldInline localDecl.userName
+def shouldInlineLocal (localDecl : LocalDecl) : SimpM Bool := do
+  match (← get).occInfo.map.find? localDecl.userName with
+  | some .once => return true
+  | _ => lcnfSizeLe localDecl.value (← read).config.smallThreshold
 
 structure InlineCandidateInfo where
   isLocal : Bool
@@ -189,8 +173,7 @@ structure InlineCandidateInfo where
 
 def inlineCandidate? (e : Expr) : SimpM (Option InlineCandidateInfo) := do
   let f := e.getAppFn
-  match f with
-  | .const declName us =>
+  if let .const declName us ← findExpr f then
     unless hasInlineAttribute (← getEnv) declName do return none
     -- TODO: check whether function is recursive or not.
     -- We can skip the test and store function inline so far.
@@ -198,35 +181,57 @@ def inlineCandidate? (e : Expr) : SimpM (Option InlineCandidateInfo) := do
     let numArgs := e.getAppNumArgs
     let arity := decl.getArity
     if numArgs < arity then return none
+    /-
+    Recall that we use binder names to build `InlineStats`.
+    Thus, we use `ensureUniqueLetVarNames` to make sure there is no name collision.
+    -/
+    let value ← ensureUniqueLetVarNames (decl.value.instantiateLevelParams decl.levelParams us)
     return some {
-      arity
+      arity, value
       isLocal := false
-      value := decl.value.instantiateLevelParams decl.levelParams us
     }
-  | _ =>
-    match (← findLambda? f) with
-    | none => return none
-    | some localDecl =>
-      unless (← shouldInline localDecl) do return none
-      let numArgs := e.getAppNumArgs
-      let arity := getLambdaArity localDecl.value
-      if numArgs < arity then return none
-      return some {
-        arity
-        isLocal := true
-        value := localDecl.value
-      }
+  else if let some localDecl ← findLambda? f then
+    unless (← shouldInlineLocal localDecl) do return none
+    let numArgs := e.getAppNumArgs
+    let arity := getLambdaArity localDecl.value
+    if numArgs < arity then return none
+    let value ← ensureUniqueLetVarNames localDecl.value
+    return some {
+      arity, value
+      isLocal := true
+    }
+  else
+    return none
 
 /--
 If `e` if a free variable that expands to a valid LCNF terminal `let`-block expression `e'`,
-return `e'`. -/
+return `e'`.
+-/
 def expandTrivialExpr (e : Expr) : SimpM Expr := do
   if e.isFVar then
     let e' ← findExpr e
     unless e'.isLambda do
-      if e != e' then markSimplified
-      return e'
+      if e != e' then
+        markSimplified
+        return e'
   return e
+
+/--
+Given `value` of the form `let x_1 := v_1; ...; let x_n := v_n; e`,
+return `let x_1; ...; let x_n := v_n; let y : type := e; body`.
+
+This methods assumes `type` and `value` do not have loose bound variables.
+
+Remark: `body` may have many loose bound variables, and the loose bound variables > 0
+must be lifted by `n`.
+-/
+def mkFlatLet (y : Name) (type : Expr) (value : Expr) (body : Expr) (nonDep : Bool := false) : Expr :=
+  go value 0
+where
+  go (value : Expr) (i : Nat) : Expr :=
+    match value with
+    | .letE n t v b d => .letE n t v (go b (i+1)) d
+    | _ => .letE y type value (body.liftLooseBVars 1 i) nonDep
 
 /--
 Auxiliary function for projecting "type class dictionary access".
@@ -260,8 +265,8 @@ partial def inlineProjInst? (e : Expr) : OptionT SimpM Expr := do
   Recall that we are extracting only one of the type class elements.
   -/
   let value ← withNewScope do mkLetUsingScope (← visitProj e)
-  /- We use `visitLet` again to put back on the current local context the relevant let-declarations. -/
-  visitLet (m := SimpM) value fun _ value => return value
+  markSimplified
+  internalize value
 where
   visitProj (e : Expr) : OptionT SimpM Expr := do
     let .proj _ i s := e | unreachable!
@@ -284,18 +289,118 @@ where
       guard <| decl.getArity == e.getAppNumArgs
       let value := decl.value.instantiateLevelParams decl.levelParams us
       let value := value.beta e.getAppArgs
-      let value ← visitLet (m := SimpM) value fun _ value => return value
+      /-
+      Here, we just go inside of the let-declaration block without trying to simplify it.
+      Reason: a type class instannce may have many elements, and it does not make sense to simplify
+      all of them when we are extracting only one of them.
+      -/
+      let value ← Compiler.visitLet (m := SimpM) value fun _ value => return value
       visit value
 
-mutual
+def betaReduce (e : Expr) (args : Array Expr) : SimpM Expr := do
+  -- TODO: add necessary casts
+  internalize (e.beta args)
 
-partial def visitLambda (e : Expr) : SimpM Expr :=
+/--
+Try "cases on cases" simplification.
+If `casesFn args` is of the form
+```
+casesOn _x.i
+  (... let _x.j₁ := ctorⱼ₁ ...; _jp.k _x.j₁)
+  ...
+  (... let _x.jₙ := ctorⱼₙ ...; _jp.k _x.jₙ)
+```
+where `_jp.k` is a join point of the form
+```
+let _jp.k := fun y =>
+  casesOn y ...
+```
+Then, inline `_jp.k`. The idea is to force the `casesOn` application in the join point to
+reduce after the inlining step.
+Example: consider the following declarations
+```
+@[inline] def pred? (x : Nat) : Option Nat :=
+  match x with
+  | 0 => none
+  | x+1 => some x
+
+def isZero (x : Nat) :=
+ match pred? x with
+ | some _ => false
+ | none => true
+```
+After inlining `pred?` in `isZero`, we have
+```
+let _jp.1 := fun y : Option Nat =>
+  casesOn y true (fun y => false)
+casesOn x
+  (let _x.1 := none; _jp.1 _x.1)
+  (fun n => let _x.2 := some n; _jp.1 _x.2)
+```
+and this simplification is applicable, producing
+```
+casesOn x true (fun n => false)
+```
+-/
+def simpCasesOnCases? (casesInfo : CasesInfo) (casesFn : Expr) (args : Array Expr) : OptionT SimpM Expr := do
+  let mut jpFirst? := none
+  for i in casesInfo.altsRange do
+    let alt := args[i]!
+    let jp ← isJpCtor? alt
+    if let some jpFirst := jpFirst? then
+       guard <| jp == jpFirst
+    else
+       let some localDecl ← findDecl? jp | failure
+       let .lam _ _ jpBody _ := localDecl.value | failure
+       guard (← isCasesApp? jpBody).isSome
+       jpFirst? := jp
+  let some jpFVarId := jpFirst? | failure
+  let some localDecl ← findDecl? jpFVarId | failure
+  let .lam _ _ jpBody _ := localDecl.value | failure
+  let mut args := args
+  for i in casesInfo.altsRange do
+    args := args.modify i (inlineJp · jpBody)
+  return mkAppN casesFn args
+where
+  isJpCtor? (alt : Expr) : OptionT SimpM FVarId := do
+    match alt with
+    | .lam _ _ b _ => isJpCtor? b
+    | .letE _ _ v b _ => match b with
+      | .letE .. => isJpCtor? b
+      | .app (.fvar fvarId) (.bvar 0) =>
+        let some localDecl ← findDecl? fvarId | failure
+        guard localDecl.isJp
+        guard <| v.isConstructorApp (← getEnv)
+        return fvarId
+      | _ => failure
+    | _ => failure
+
+  inlineJp (alt : Expr) (jpBody : Expr) : Expr :=
+    match alt with
+    | .lam n d b bi => .lam n d (inlineJp b jpBody) bi
+    | .letE n t v b nd => .letE n t v (inlineJp b jpBody) nd
+    | _ => jpBody
+
+mutual
+/--
+Simplify the given lambda expression.
+If `checkEmptyTypes := true`, then return `fun a_i : t_i => lcUnreachable` if
+`t_i` is the `Empty` type.
+-/
+partial def visitLambda (e : Expr) (checkEmptyTypes := false): SimpM Expr :=
   withNewScope do
     let (as, e) ← Compiler.visitLambda e
+    if checkEmptyTypes then
+      for a in as do
+        if (← isEmptyType (← inferType a)) then
+          let unreach ← mkLcUnreachable (← inferType e)
+          let r ← mkLambda as unreach
+          return r
     let e ← mkLetUsingScope (← visitLet e)
     mkLambda as e
 
 partial def visitCases (casesInfo : CasesInfo) (e : Expr) : SimpM Expr := do
+  let f := e.getAppFn
   let mut args  := e.getAppArgs
   let major := args[casesInfo.discrsRange.stop - 1]!
   let major ← findExpr major
@@ -308,10 +413,12 @@ partial def visitCases (casesInfo : CasesInfo) (e : Expr) : SimpM Expr := do
     assert! !alt.isLambda
     markSimplified
     visitLet alt
+  else if let some e ← simpCasesOnCases? casesInfo f args then
+    visitCases casesInfo e
   else
     for i in casesInfo.altsRange do
-      args ← args.modifyM i visitLambda
-    return mkAppN e.getAppFn args
+      args ← args.modifyM i (visitLambda · (checkEmptyTypes := true))
+    return mkAppN f args
 
 /--
 If `e` is an application that can be inlined, inline it.
@@ -326,56 +433,51 @@ partial def inlineApp? (e : Expr) (xs : Array Expr) (k? : Option Expr) : SimpM (
   let numArgs := args.size
   trace[Compiler.simp.inline] "inlining {e}"
   markSimplified
-  withLocalInline info.isLocal do
-  if !(← manyExitPoints info.value) then
-    -- If `info.value` has only one exit point, we don't need to create a new join point
-    let value := info.value.beta args[:info.arity]
-    let value ← visitLet value #[]
-    match numArgs == info.arity, k? with
-      | true, none => return value
-      | false, none => return mkAppN (← mkAuxLetDecl value) args[info.arity:]
-      | true, some k => let x ← mkAuxLetDecl value; visitLet k (xs.push x)
-      | false, some k =>
-        let x ← mkAuxLetDecl value
-        let x ← mkAuxLetDecl (mkAppN x args[info.arity:])
-        visitLet k (xs.push x)
+  if k?.isNone && numArgs == info.arity then
+    /- Easy case, there is no continuation and `e` is not over applied -/
+    visitLet (← betaReduce info.value args)
+  else if (← onlyOneExitPoint info.value) then
+    /- If `info.value` has only one exit point, we don't need to create a new auxiliary join point -/
+    let mut value ← betaReduce info.value args[:info.arity]
+    if numArgs > info.arity then
+      let type ← inferType (mkAppN e.getAppFn args[:info.arity])
+      value := mkFlatLet (← mkAuxLetDeclName) type value (mkAppN (.bvar 0) args[info.arity:])
+    if let some k := k? then
+      let type ← inferType e
+      value := mkFlatLet (← mkAuxLetDeclName) type value k
+    visitLet value xs
   else
-    let args := e.getAppArgs
-    if k?.isNone && numArgs == info.arity then
-      -- Easy case, there is no continuation and `e` is not overapplied
-      return info.value.beta args
-    else
-      /-
-      There is a continuation `k` or `e` is over applied.
-      If `e` is over applied, the extra arguments act as a continuation.
+    /-
+    There is a continuation `k` or `e` is over applied.
+    If `e` is over applied, the extra arguments act as a continuation.
 
-      We create a new join point
-      ```
-      let jp := fun y =>
-        let x := y <extra-arguments> -- if `e` is over applied
-        k
-      ```
-      Recall that `visitLet` incorporates the current continuation
-      to the new join point `jp`.
-      -/
-      let jpDomain ← inferType (mkAppN e.getAppFn args[:info.arity])
-      let binderName ← mkFreshUserName `_y
-      let jp ← withNewScope do
-        let y ← mkLocalDecl binderName jpDomain
-        let body ← if numArgs == info.arity then
-          visitLet k?.get! (xs.push y)
+    We create a new join point
+    ```
+    let jp := fun y =>
+      let x := y <extra-arguments> -- if `e` is over applied
+      k
+    ```
+    Recall that `visitLet` incorporates the current continuation
+    to the new join point `jp`.
+    -/
+    let jpDomain ← inferType (mkAppN e.getAppFn args[:info.arity])
+    let binderName ← mkFreshUserName `_y
+    let jp ← withNewScope do
+      let y ← mkLocalDecl binderName jpDomain
+      let body ← if numArgs == info.arity then
+        visitLet k?.get! (xs.push y)
+      else
+        let x ← mkAuxLetDecl (mkAppN y args[info.arity:])
+        if let some k := k? then
+          visitLet k (xs.push x)
         else
-          let x ← mkAuxLetDecl (mkAppN y args[info.arity:])
-          if let some k := k? then
-            visitLet k (xs.push x)
-          else
-            visitLet x (xs.push x)
-        let body ← mkLetUsingScope body
-        mkLambda #[y] body
-      let jp ← mkJpDeclIfNotSimple jp
-      let value := info.value.beta args[:info.arity]
-      let value ← attachJp value jp
-      visitLet value
+          visitLet x (xs.push x)
+      let body ← mkLetUsingScope body
+      mkLambda #[y] body
+    let jp ← mkJpDeclIfNotSimple jp
+    let value ← betaReduce info.value args[:info.arity]
+    let value ← attachJp value jp
+    visitLet value
 
 /-- Try to apply simple simplifications. -/
 partial def simpValue? (e : Expr) : SimpM (Option Expr) :=
@@ -392,6 +494,10 @@ partial def visitLet (e : Expr) (xs : Array Expr := #[]): SimpM Expr := do
     if value.isLambda then
       value ← visitLambda value
     else if let some value' ← simpValue? value then
+      if value'.isLet then
+        let e := mkFlatLet binderName type value' body nonDep
+        let e ← visitLet e xs
+        return e
       value := value'
     if value.isFVar then
       /- Eliminate `let _x_i := _x_j;` -/
@@ -405,8 +511,9 @@ partial def visitLet (e : Expr) (xs : Array Expr := #[]): SimpM Expr := do
       visitLet body (xs.push x)
   | _ =>
     let e := e.instantiateRev xs
-    let e := (← simpValue? e).getD e
-    if let some casesInfo ← isCasesApp? e then
+    if let some value ← simpValue? e then
+      visitLet value
+    else if let some casesInfo ← isCasesApp? e then
       visitCases casesInfo e
     else if let some e ← inlineApp? e #[] none then
       return e
@@ -416,20 +523,20 @@ end
 
 end Simp
 
-def Decl.simp? (decl : Decl) : CoreM (Option Decl) := do
-  let decl ← decl.ensureUniqueLetVarNames
-  let stats ← Simp.collectInlineStats decl.value
-  trace[Compiler.simp.inline.stats] "{decl.name}:{Format.nest 2 (format stats)}"
-  let (value, s) ← Simp.visitLambda decl.value |>.run { stats } |>.run { simplified := false } |>.run' {}
+def Decl.simp? (decl : Decl) : Simp.SimpM (Option Decl) := do
+  let value ← Simp.internalize decl.value
+  trace[Compiler.simp.inline.occs] "{decl.name}:{Format.nest 2 (format (← get).occInfo)}"
   trace[Compiler.simp.step] "{decl.name} :=\n{decl.value}"
+  let value ← Simp.visitLambda value
+  trace[Compiler.simp.step.new] "{decl.name} :=\n{value}"
   trace[Compiler.simp.stat] "{decl.name}: {← getLCNFSize decl.value}"
-  if s.simplified then
+  if (← get).simplified then
     return some { decl with value }
   else
     return none
 
 partial def Decl.simp (decl : Decl) : CoreM Decl := do
-  if let some decl ← decl.simp? then
+  if let some decl ← decl.simp? |>.run {} |>.run' {} |>.run' {} then
     -- TODO: bound number of steps?
     decl.simp
   else
@@ -439,6 +546,7 @@ builtin_initialize
   registerTraceClass `Compiler.simp.inline
   registerTraceClass `Compiler.simp.stat
   registerTraceClass `Compiler.simp.step
-  registerTraceClass `Compiler.simp.inline.stats
+  registerTraceClass `Compiler.simp.step.new
+  registerTraceClass `Compiler.simp.inline.occs
 
 end Lean.Compiler
